Fixing merge conflict

src/Experiments/Ed25519.v
@@ -7,12 +7,18 @@ Require Crypto.Encoding.PointEncoding.
 Import Morphisms.
 
 Context {H: forall n : nat, Word.word n -> Word.word (b + b)}.
+(* TODO : define feSign *)
 Context {feSign : GF25519.fe25519 -> bool}.
+Context {feSign_correct : forall x,
+            PointEncoding.sign x = feSign (ModularBaseSystem.encode x)}.
+Context {Proper_feSign :  Proper (ModularBaseSystem.eq ==> eq) feSign}.
 
 Definition a : GF25519.fe25519 :=
   Eval vm_compute in ModularBaseSystem.encode a.
 Definition d : GF25519.fe25519 :=
   Eval vm_compute in ModularBaseSystem.encode d.
+Definition twice_d : GF25519.fe25519 :=
+  Eval vm_compute in (GF25519.add d d).
 
 Lemma phi_a : ModularBaseSystem.eq (ModularBaseSystem.encode Ed25519.a) a.
 Proof. reflexivity. Qed.
@@ -31,44 +37,19 @@ Let Erep := (@ExtendedCoordinates.Extended.point
          d
       ).
 
-
-Global Instance Proper_onCurve {F eq one add mul a d} :
-  Proper (Tuple.fieldwise (n := 2) eq==> iff) (@Pre.onCurve F eq one add mul a d) | 0.
+(* TODO : prove -- use Ed25519.curve25519_params_ok *)
+Lemma twedprm_ERep :
+  @CompleteEdwardsCurve.E.twisted_edwards_params
+   GF25519.fe25519 ModularBaseSystem.eq
+   GF25519.zero_ GF25519.one_
+   GF25519.add GF25519.mul a d.
+Proof.
 Admitted.
 
-Definition coord_to_extended (xy :  GF25519.fe25519 * GF25519.fe25519) : @Pre.onCurve _ (@ModularBaseSystem.eq GF25519.modulus
-                           GF25519.params25519)
-                        (@ModularBaseSystem.one GF25519.modulus
-                           GF25519.params25519) GF25519.add
-                        GF25519.mul a d xy -> Erep.
-Proof.
-  intros.
-  destruct xy as [X Y].
-  exists (X, Y, GF25519.one_, GF25519.mul X Y).
-  repeat split.
-  + cbv [ModularBaseSystem.div].
-    rewrite !(@Algebra.Field.div_one _ _ _ _ _ _ _ _ _ _ (PrimeFieldTheorems.F.field_modulo GF25519.modulus)).
-    match goal with H: Pre.onCurve (?X1, ?Y1) |- Pre.onCurve (?X2, ?Y2) =>
-                    assert (Tuple.fieldwise (n := 2) ModularBaseSystem.eq (X2, Y2) (X1, Y1)) by (econstructor; cbv [fst snd Tuple.fieldwise' ModularBaseSystem.eq]; apply ModularBaseSystemProofs.encode_rep) end.
-    pose proof @Proper_onCurve.
-    cbv [Proper respectful] in *.
-    match goal with H: Tuple.fieldwise _ ?x ?y, H1: Pre.onCurve ?y |- _  =>
-                    pose proof (proj2
-                                  (@Proper_onCurve _
-                                  ModularBaseSystem.eq
-                                  GF25519.one_
-                                  GF25519.add
-                                  GF25519.mul
-                                  a d x y H) H1) end.
-    assumption.
-  + intro A. symmetry in A.
-    apply (Algebra.field_is_zero_neq_one (field := GF25519.field25519)).
-    rewrite GF25519.one_subst, GF25519.zero_subst.
-    auto.
-  + pose proof GF25519.field25519.
-    rewrite (Algebra.left_identity (id := GF25519.one_)).
-    reflexivity.
-Defined.
+Definition coord_to_extended (xy : GF25519.fe25519 * GF25519.fe25519) pf :=
+  ExtendedCoordinates.Extended.from_twisted
+    (field := GF25519.field25519) (prm :=twedprm_ERep)
+    (exist Pre.onCurve xy pf).
 
 Definition extended_to_coord (P : Erep) : (GF25519.fe25519 * GF25519.fe25519) :=
   CompleteEdwardsCurve.E.coordinates (ExtendedCoordinates.Extended.to_twisted P).
@@ -95,8 +76,15 @@ Let EToRep := PointEncoding.point_phi
 .
 
 Let ZNWord sz x := Word.NToWord sz (BinInt.Z.to_N x).
+Let WordNZ {sz} (w : Word.word sz) := BinInt.Z.of_N (Word.wordToN w).
 
-Definition feEnc (x : GF25519.fe25519) : Word.word 255 :=
+(* TODO : 
+   GF25519.pack does most of the work here, but the spec currently talks
+   about 256-bit words and [pack] makes a sequence of short (in this case
+   32- and 31-bit) Zs. We should either automate this transformation or change
+   the spec.
+ *)
+Definition feEnc (x : GF25519.fe25519) : Word.word 255 := 
   let '(x0, x1, x2, x3, x4, x5, x6, x7) :=
       (GF25519.pack x) in
   Word.combine (ZNWord 32 x0)
@@ -106,6 +94,25 @@ Definition feEnc (x : GF25519.fe25519) : Word.word 255 :=
           (Word.combine (ZNWord 32 x4)
             (Word.combine (ZNWord 32 x5)
               (Word.combine (ZNWord 32 x6) (ZNWord 31 x7))))))).
+
+Definition feDec (w : Word.word 255) : option GF25519.fe25519 :=
+  let w0 := Word.split1 32 _ w in
+  let a0 := Word.split2 32 _ w in
+  let w1 := Word.split1 32 _ a0 in
+  let a1 := Word.split2 32 _ a0 in
+  let w2 := Word.split1 32 _ a1 in
+  let a2 := Word.split2 32 _ a1 in
+  let w3 := Word.split1 32 _ a2 in
+  let a3 := Word.split2 32 _ a2 in
+  let w4 := Word.split1 32 _ a3 in
+  let a4 := Word.split2 32 _ a3 in
+  let w5 := Word.split1 32 _ a4 in
+  let a5 := Word.split2 32 _ a4 in
+  let w6 := Word.split1 32 _ a5 in
+  let w7 := Word.split2 32 _ a5 in
+  let result := (GF25519.unpack (WordNZ w0, WordNZ w1, WordNZ w2, WordNZ w3, WordNZ w4, WordNZ w5, WordNZ w6, WordNZ w7)) in
+  if GF25519.ge_modulus result
+  then None else (Some result).
 
 Let ERepEnc :=
   (PointEncoding.Kencode_point
@@ -123,8 +130,77 @@ Let S2Rep := fun (x : ModularArithmetic.F.F l) =>
                   (List.repeat (BinInt.Z.of_nat 32) 8)
                   (ModularArithmetic.F.to_Z x))).
 
+Lemma eq_a_minus1 : ModularBaseSystem.eq a (GF25519.opp GF25519.one_).
+Proof.
+  etransitivity; [ symmetry; apply phi_a | ].
+  cbv [ModularBaseSystem.eq].
+  rewrite GF25519.opp_correct.
+  rewrite ModularBaseSystemOpt.opp_opt_correct.
+  rewrite ModularBaseSystemProofs.opp_rep with (x := ModularArithmetic.F.one) by reflexivity.
+  apply ModularBaseSystemProofs.encode_rep.
+Qed.
 
+About ExtendedCoordinates.Extended.add.
+Let ErepAdd :=
+  (@ExtendedCoordinates.Extended.add _ _ _ _ _ _ _ _ _ _
+                                     a d GF25519.field25519 twedprm_ERep _
+                                     eq_a_minus1 twice_d (eq_refl _) ).
 
+(* TODO : unclear what we're doing with the placeholder [feEnc] at the moment, so
+   leaving this admitted for now *)
+Lemma feEnc_correct : forall x,
+    PointEncoding.Fencode x = feEnc (ModularBaseSystem.encode x).
+Admitted.
+
+(* TODO : unclear what we're doing with the placeholder [feEnc] at the moment, so
+   leaving this admitted for now *)
+Lemma Proper_feEnc : Proper (ModularBaseSystem.eq ==> eq) feEnc.
+Admitted.
+
+Lemma ext_to_coord_coord_to_ext : forall (P : GF25519.fe25519 * GF25519.fe25519)
+                                         (pf : Pre.onCurve P),
+               Tuple.fieldwise (n := 2)
+                 ModularBaseSystem.eq
+                 (extended_to_coord (coord_to_extended P pf))
+                 P.
+Proof.
+  cbv [extended_to_coord coord_to_extended].
+  intros.
+  transitivity (CompleteEdwardsCurve.E.coordinates (exist _ P pf));
+    [ | reflexivity].
+  apply (CompleteEdwardsCurveTheorems.E.Proper_coordinates
+           (field := GF25519.field25519) (a := a) (d := d)).
+  apply ExtendedCoordinates.Extended.to_twisted_from_twisted.
+Qed.
+
+Lemma ERepEnc_correct P : Eenc P = ERepEnc (EToRep P).
+Proof.
+  cbv [Eenc ERepEnc EToRep sign Fencode].
+  transitivity (PointEncoding.encode_point (b := 255) P);
+    [ | apply (PointEncoding.Kencode_point_correct
+           (Ksign_correct := feSign_correct)
+           (Kenc_correct := feEnc_correct)
+           (Kp2c_c2p := ext_to_coord_coord_to_ext)
+           (Proper_Ksign := Proper_feSign)
+           (Proper_Kenc := Proper_feEnc))
+    ].
+  reflexivity.
+Qed.
+
+Lemma ext_eq_correct : forall p q : Erep,
+  ExtendedCoordinates.Extended.eq p q <->
+  Tuple.fieldwise (n := 2) ModularBaseSystem.eq (extended_to_coord p) (extended_to_coord q).
+Proof.
+  cbv [extended_to_coord]; intros.
+  cbv [ExtendedCoordinates.Extended.eq].
+  match goal with |- _ <-> Tuple.fieldwise _
+                                           (CompleteEdwardsCurve.E.coordinates ?x)
+                                           (CompleteEdwardsCurve.E.coordinates ?y) =>
+                  pose proof (CompleteEdwardsCurveTheorems.E.Proper_coordinates
+                                (field := GF25519.field25519) (a := a) (d := d) x y)
+  end.
+  tauto.
+Qed.
 
 Check @sign_correct
       (* E := *) E
@@ -144,14 +220,14 @@ Check @sign_correct
       (* prm := *) ed25519
       (* Erep := *) Erep
       (* ErepEq := *) ExtendedCoordinates.Extended.eq
-      (* ErepAdd := *) ExtendedCoordinates.Extended.add
+      (* ErepAdd := *) ErepAdd
       (* ErepId := *) ExtendedCoordinates.Extended.zero
       (* ErepOpp := *) ExtendedCoordinates.Extended.opp
       (* Agroup := *) ExtendedCoordinates.Extended.extended_group
       (* EToRep := *) EToRep
       (* ERepEnc := *) ERepEnc
-      (* ERepEnc_correct := *) PointEncoding.Kencode_point_correct
-      (* Proper_ERepEnc := *) PointEncoding.Proper_Kencode_point
+      (* ERepEnc_correct := *) ERepEnc_correct
+      (* Proper_ERepEnc := *) (PointEncoding.Proper_Kencode_point (Kpoint_eq_correct := ext_eq_correct) (Proper_Kenc := Proper_feEnc))
       (* SRep := *) (Tuple.tuple (Word.word 32) 8)
       (* SRepEq := *) (Tuple.fieldwise Logic.eq)
       (* H0 := *) Tuple.Equivalence_fieldwise
@@ -170,10 +246,115 @@ Check @sign_correct
       (* SRepMul := *) _
       (* SRepMul_correct := *) _
       (* Proper_SRepMul := *) _
-      (* ErepB := *) _
+      (* ErepB := *) (EToRep B)
       (* ErepB_correct := *) _
       (* SRepDecModLShort := *) _
       (* SRepDecModLShort_correct := *) _
-      .
+.
+
+Definition Fsqrt_minus1 := Eval vm_compute in ModularBaseSystem.decode (GF25519.sqrt_m1).
+Definition Fsqrt := PrimeFieldTheorems.F.sqrt_5mod8 Fsqrt_minus1.
+Lemma bound_check255 : BinInt.Z.to_nat GF25519.modulus < PeanoNat.Nat.pow 2 255.
+Proof.
+  cbv [GF25519.modulus].
+  rewrite <-(Znat.Nat2Z.id 2) at 1.
+  rewrite ZUtil.Z.pow_Z2N_Zpow by Omega.omega.
+  apply Znat.Z2Nat.inj_lt; cbv; congruence.
+Qed.
+
+Lemma bound_check256 : BinInt.Z.to_nat GF25519.modulus < PeanoNat.Nat.pow 2 256.
+Proof.
+  cbv [GF25519.modulus].
+  rewrite <-(Znat.Nat2Z.id 2) at 1.
+  rewrite ZUtil.Z.pow_Z2N_Zpow by Omega.omega.
+  apply Znat.Z2Nat.inj_lt; cbv; congruence.
+Qed.
+
+Let Edec := (@PointEncodingPre.point_dec
+               _ eq
+               ModularArithmetic.F.zero
+               ModularArithmetic.F.one
+               ModularArithmetic.F.opp
+               ModularArithmetic.F.add
+               ModularArithmetic.F.sub
+               ModularArithmetic.F.mul
+               ModularArithmetic.F.div
+               _
+               Ed25519.a
+               Ed25519.d
+               _
+               Fsqrt
+               (PointEncoding.Fencoding (bound_check := bound_check255))
+               sign).
+
+Let Sdec : Word.word b -> option (ModularArithmetic.F.F l) :=
+ fun w =>
+ let z := (BinIntDef.Z.of_N (Word.wordToN w)) in
+ if ZArith_dec.Z_lt_dec z l
+ then Some (ModularArithmetic.F.of_Z l z) else None.
+
+Let ERepDec :=
+    (@PointEncoding.Kdecode_point
+         _
+         GF25519.fe25519
+         ModularBaseSystem.eq
+         GF25519.zero_
+         GF25519.one_
+         GF25519.opp
+         GF25519.add
+         GF25519.sub
+         GF25519.mul
+         ModularBaseSystem.div
+         _ a d feSign
+         _ coord_to_extended
+         feDec GF25519.sqrt
+       ).
 
 Check verify_correct.
+Check @verify_correct
+      (* E := *) E
+      (* Eeq := *) CompleteEdwardsCurveTheorems.E.eq
+      (* Eadd := *) CompleteEdwardsCurve.E.add
+      (* Ezero := *) CompleteEdwardsCurve.E.zero
+      (* Eopp := *) CompleteEdwardsCurveTheorems.E.opp
+      (* EscalarMult := *) CompleteEdwardsCurve.E.mul
+      (* b := *) b
+      (* H := *) H
+      (* c := *) c
+      (* n := *) n
+      (* l := *) l
+      (* B := *) B
+      (* Eenc := *) Eenc
+      (* Senc := *) Senc
+      (* prm := *) ed25519
+      (* Proper_Eenc := *) PointEncoding.Proper_encode_point
+      (* Edec := *) Edec
+      (* eq_enc_E_iff := *) _
+      (* Sdec := *) Sdec
+      (* eq_enc_S_iff := *) _
+      (* Erep := *) Erep
+      (* ErepEq := *) ExtendedCoordinates.Extended.eq
+      (* ErepAdd := *) ErepAdd
+      (* ErepId := *) ExtendedCoordinates.Extended.zero
+      (* ErepOpp := *) ExtendedCoordinates.Extended.opp
+      (* Agroup := *) ExtendedCoordinates.Extended.extended_group
+      (* EToRep := *) EToRep
+      (* Ahomom := *) _
+      (* ERepEnc := *) ERepEnc
+      (* ERepEnc_correct := *) ERepEnc_correct
+      (* Proper_ERepEnc := *) (PointEncoding.Proper_Kencode_point (Kpoint_eq_correct := ext_eq_correct) (Proper_Kenc := Proper_feEnc))
+      (* ERepDec := *) ERepDec
+      (* ERepDec_correct := *) _
+      (* SRep := *) (Tuple.tuple (Word.word 32) 8)
+      (* SRepEq := *) (Tuple.fieldwise Logic.eq)
+      (* H0 := *) Tuple.Equivalence_fieldwise
+      (* S2Rep := *) S2Rep
+      (* SRepDecModL := *) _
+      (* SRepDecModL_correct := *) _
+      (* SRepERepMul := *) _
+      (* SRepERepMul_correct := *) _
+      (* Proper_SRepERepMul := *) _
+      (* SRepDec := *) _
+      (* SRepDec_correct := *) _
+      (* mlen := *) _
+      .
